[WIP] [Dafny] Make progress with proof for from_exp

compiler/dafny_new/semantics/dafny_compilerProofScript.sml
@@ -3,6 +3,7 @@
 *)
 
 open preamble
+open astTheory
 open semanticPrimitivesTheory
 open evaluateTheory
 open dafny_semanticPrimitivesTheory
@@ -10,6 +11,7 @@ open dafny_evaluateTheory
 open namespaceTheory
 open mlstringTheory
 open integerTheory
+open mlintTheory
 
 (* For compiler definitions *)
 open result_monadTheory
@@ -46,10 +48,6 @@ End
 
 Definition cml_get_arr_data_def:
   cml_get_arr_data cml_e = cml_tup_select 2 cml_e 1
-End
-
-Definition cml_arr_sel_def:
-  cml_arr_sel cml_arr cml_idx = App Asub [cml_get_arr_data cml_arr; cml_idx]
 End
 
 Definition cml_fapp_aux_def:
@@ -140,7 +138,7 @@ Definition from_exp_def:
   do
     cml_e₀ <- from_exp e₀;
     cml_e₁ <- from_exp e₁;
-    (* Force left-to-right order *)
+    (* Force left-to-right evaluation order *)
     n_e₀ <<- " l";
     return (Let (SOME n_e₀) cml_e₀
              (from_bin_op bop (Var (Short n_e₀)) cml_e₁))
@@ -154,7 +152,10 @@ Definition from_exp_def:
   do
     cml_arr <- from_exp arr;
     cml_idx <- from_exp idx;
-    return (cml_arr_sel cml_arr cml_idx)
+    (* Force left-to-right evaluation order *)
+    n_arr <<- " arr";
+    return (Let (SOME n_arr) cml_arr
+                (App Asub [cml_get_arr_data (Var (Short n_arr)); cml_idx]))
   od ∧
   from_exp (FunCall n args) =
   do
@@ -182,7 +183,7 @@ Type dfy_env[pp] = “:dafny_semanticPrimitives$sem_env”
 Type dfy_exp[pp] = “:dafny_ast$exp”
 Type dfy_exp_res[pp] = “:'a dafny_semanticPrimitives$exp_result”
 
-Type cml_state[pp] = “:α semanticPrimitives$state”
+Type cml_state[pp] = “:'ffi semanticPrimitives$state”
 Type cml_env[pp] = “:v semanticPrimitives$sem_env”
 Type cml_exp[pp] = “:ast$exp”
 Type cml_res[pp] = “:(v list, v) semanticPrimitives$result”
@@ -280,6 +281,8 @@ Proof
   gvs [state_rel_def, locals_rel_def]
 QED
 
+(* TODO Is defining these + manually using drule really the way one does
+   this? *)
 Triviality exp_res_rel_rval:
   exp_res_rel m (Rval dfy_v) r_cml ⇒ ∃cml_v. r_cml = Rval [cml_v]
 Proof
@@ -296,6 +299,23 @@ Proof
   \\ namedCases_on ‘err’ ["raise", "abort"] \\ gvs []
   \\ Cases_on ‘abort’ \\ gvs []
   \\ Cases_on ‘dfy_err’ \\ gvs []
+QED
+
+Triviality exp_ress_rel_rerr:
+  exp_ress_rel m (Rerr dfy_err) rs_cml ⇒
+  dfy_err = Rtimeout_error ∧ rs_cml = (Rerr (Rabort Rtimeout_error))
+Proof
+  namedCases_on ‘rs_cml’ ["vs", "err"] \\ gvs []
+  \\ namedCases_on ‘err’ ["raise", "abort"] \\ gvs []
+  \\ Cases_on ‘abort’ \\ gvs []
+  \\ Cases_on ‘dfy_err’ \\ gvs []
+QED
+
+Triviality exp_ress_rel_rval:
+  exp_ress_rel m (Rval dfy_vs) rs_cml ⇒
+  ∃cml_vs. rs_cml = Rval cml_vs ∧ LIST_REL (val_rel m) dfy_vs cml_vs
+Proof
+  namedCases_on ‘rs_cml’ ["vs", "err"] \\ gvs []
 QED
 
 (* NOTE If we have multiple of these, can abstract aways into a function that
@@ -370,7 +390,7 @@ Proof
 QED
 
 Triviality state_rel_flookup_m:
-  state_rel m l s' t' env_cml ∧
+  state_rel m l s t env_cml ∧
   FLOOKUP m dfy_loc = SOME cml_loc ∧
   FLOOKUP m dfy_loc' = SOME cml_loc' ⇒
   ((cml_loc' = cml_loc) ⇔ (dfy_loc' = dfy_loc))
@@ -378,26 +398,46 @@ Proof
   cheat
 QED
 
+Triviality state_rel_llookup:
+  state_rel m l s t env_cml ∧
+  LLOOKUP s.heap dfy_loc = SOME (HArr dfy_arr) ∧
+  FLOOKUP m dfy_loc = SOME cml_loc ⇒
+  ∃cml_arr.
+    store_lookup cml_loc t.refs = SOME (Varray cml_arr) ∧
+    LIST_REL (val_rel m) dfy_arr cml_arr
+Proof
+  cheat
+QED
+
+(* TODO Upstream to HOL? *)
+Triviality LIST_REL_EL:
+  LIST_REL R l1 l2 ⇔ (∀i. i < LENGTH l1 ⇒ R (EL i l1) (EL i l2))
+Proof
+  cheat
+QED
+
 Theorem correct_from_exp:
-  (∀s env_dfy e_dfy s' r_dfy t env_cml e_cml m l.
+  (∀s env_dfy e_dfy s' r_dfy (t: 'ffi cml_state) env_cml e_cml m l.
      evaluate_exp s env_dfy e_dfy = (s', r_dfy) ∧
      from_exp e_dfy = INR e_cml ∧ state_rel m l s t env_cml ∧
      env_rel env_dfy env_cml ∧ valid_name e_dfy ∧
      r_dfy ≠ Rerr Rtype_error
-     ⇒ ∃t' r_cml.
+     ⇒ ∃(t': 'ffi cml_state) r_cml.
          evaluate$evaluate t env_cml [e_cml] = (t', r_cml) ∧
          state_rel m l s' t' env_cml ∧ exp_res_rel m r_dfy r_cml) ∧
-  (∀s env_dfy es_dfy s' rs_dfy t env_cml es_cml m l.
+  (∀s env_dfy es_dfy s' rs_dfy (t: 'ffi cml_state) env_cml es_cml m l.
      evaluate_exps s env_dfy es_dfy = (s', rs_dfy) ∧
      map_from_exp es_dfy = INR es_cml ∧ state_rel m l s t env_cml ∧
      env_rel env_dfy env_cml ∧ EVERY valid_name es_dfy ∧
      rs_dfy ≠ Rerr Rtype_error
-     ⇒ ∃t' rs_cml.
+     ⇒ ∃(t': 'ffi cml_state) rs_cml.
          evaluate$evaluate t env_cml es_cml = (t', rs_cml) ∧
          state_rel m l s' t' env_cml ∧ exp_ress_rel m rs_dfy rs_cml)
 Proof
   ho_match_mp_tac evaluate_exp_ind
   \\ rpt strip_tac
+  >~ [‘Forall var term’] >-
+   (gvs [from_exp_def])
   >~ [‘Lit l’] >-
    (Cases_on ‘l’
     \\ gvs [from_exp_def, from_lit_def, evaluate_def, do_con_check_def,
@@ -521,7 +561,86 @@ Proof
       \\ gvs [from_bin_op_def]
       \\ gvs [evaluate_def, do_app_def, opb_lookup_def, opn_lookup_def,
               do_log_def, do_if_def])
-  \\ cheat
+  >~ [‘ArrLen arr’] >-
+   (gvs [from_exp_def, oneline bind_def, AllCaseEqs()]
+    \\ gvs [evaluate_exp_def]
+    \\ namedCases_on ‘evaluate_exp s env_dfy arr’ ["s₁ r"] \\ gvs []
+    \\ Cases_on ‘r = Rerr Rtype_error’ \\ gvs []
+    \\ last_x_assum drule_all \\ rpt strip_tac
+    \\ reverse $ namedCases_on ‘r’ ["arr_v",  "err"] \\ gvs []
+    >- (drule exp_res_rel_rerr
+        \\ gvs [cml_get_arr_dim_def, cml_tup_select_def, cml_tup_case_def,
+                evaluate_def])
+    \\ namedCases_on ‘get_array_len arr_v’ ["", "len"] \\ gvs []
+    \\ gvs [oneline get_array_len_def, AllCaseEqs()]
+    \\ drule exp_res_rel_rval \\ rpt strip_tac \\ gvs []
+    \\ gvs [cml_get_arr_dim_def, cml_tup_select_def, cml_tup_case_def]
+    \\ gvs [evaluate_def, can_pmatch_all_def, pmatch_def, pat_bindings_def,
+            cml_tup_vname_def, num_to_str_11]
+    \\ Cases_on ‘env_cml.v’
+    \\ gvs [alist_to_ns_def, nsAppend_def, nsLookup_def, num_to_str_11])
+  >~ [‘ArrSel arr idx’] >-
+   (gvs [from_exp_def, oneline bind_def, AllCaseEqs()]
+    \\ gvs [evaluate_exp_def]
+    \\ namedCases_on ‘evaluate_exp s env_dfy arr’ ["s₁ r"] \\ gvs []
+    \\ Cases_on ‘r = Rerr Rtype_error’ \\ gvs []
+    \\ first_x_assum drule_all \\ rpt strip_tac
+    \\ reverse $ namedCases_on ‘r’ ["arr_v",  "err"] \\ gvs []
+    >- (drule exp_res_rel_rerr \\ rpt strip_tac \\ gvs []
+        \\ gvs [cml_get_arr_data_def, cml_tup_select_def, cml_tup_case_def]
+        \\ gvs [evaluate_def])
+    \\ drule exp_res_rel_rval \\ rpt strip_tac \\ gvs []
+    \\ gvs [evaluate_def]
+    \\ rename [‘val_rel _ dfy_arr cml_arr’]
+    \\ namedCases_on ‘evaluate_exp s₁ env_dfy idx’ ["s₂ r"] \\ gvs []
+    \\ Cases_on ‘r = Rerr Rtype_error’ \\ gvs []
+    \\ ‘" " ≼ " arr"’ by gvs []  \\ drule_all state_rel_env_push_internal
+    \\ disch_then $ qspec_then ‘cml_arr’ assume_tac
+    \\ last_x_assum drule
+    \\ impl_tac >- gvs [env_rel_def]
+    \\ rpt strip_tac
+    \\ drule_all state_rel_env_pop_internal \\ rpt strip_tac \\ gvs []
+    \\ reverse $ namedCases_on ‘r’ ["idx_v",  "err"] \\ gvs []
+    >- (drule exp_res_rel_rerr \\ gvs [])
+    \\ drule exp_res_rel_rval \\ rpt strip_tac \\ gvs []
+    \\ namedCases_on ‘index_array s₂ dfy_arr idx_v’ ["", "elem"] \\ gvs []
+    \\ gvs [oneline index_array_def, oneline val_to_num_def, CaseEq "value",
+            CaseEq "option", CaseEq "heap_value"]
+    \\ gvs [cml_get_arr_data_def, cml_tup_select_def, cml_tup_case_def]
+    \\ gvs [evaluate_def, can_pmatch_all_def, pmatch_def, cml_tup_vname_def,
+            pat_bindings_def, num_to_str_11]
+    \\ Cases_on ‘env_cml.v’ \\ gvs []
+    \\ gvs [nsOptBind_def, nsBind_def, alist_to_ns_def, nsAppend_def,
+            nsLookup_def]
+    \\ gvs [do_app_def]
+    \\ drule_all state_rel_llookup \\ rpt strip_tac \\ gvs []
+    \\ gvs [INT_ABS]
+    \\ drule LIST_REL_LENGTH \\ rpt strip_tac
+    \\ gvs [LLOOKUP_EQ_EL, LIST_REL_EL])
+  >~ [‘FunCall name args’] >-
+   (cheat)
+  >~ [‘map_from_exp []’] >-
+   (gvs [from_exp_def, evaluate_exp_def, evaluate_def])
+  >~ [‘map_from_exp (e::es)’] >-
+   (gvs [from_exp_def, oneline bind_def, AllCaseEqs()]
+    \\ gvs [evaluate_exp_def]
+    \\ namedCases_on ‘evaluate_exp s env_dfy e’ ["s₁ r"] \\ gvs []
+    \\ Cases_on ‘r = Rerr Rtype_error’ \\ gvs []
+    \\ first_x_assum drule_all \\ rpt strip_tac \\ gvs []
+    \\ reverse $ namedCases_on ‘r’ ["cml_e",  "err"] \\ gvs []
+    >- (drule exp_res_rel_rerr \\ rpt strip_tac \\ gvs []
+        \\ rename [‘_::cml_es’]
+        \\ Cases_on ‘cml_es’ \\ gvs [evaluate_def])
+    \\ drule exp_res_rel_rval \\ rpt strip_tac \\ gvs []
+    \\ namedCases_on ‘es’ ["", "e' es"] \\ gvs []
+    >- (gvs [evaluate_exp_def, from_exp_def])
+    \\ namedCases_on ‘evaluate_exps s₁ env_dfy (e'::es')’ ["s₂ r"] \\ gvs []
+    \\ Cases_on ‘r = Rerr Rtype_error’ \\ gvs []
+    \\ gvs [from_exp_def, oneline bind_def, CaseEq "sum"]
+    \\ last_x_assum drule_all \\ rpt strip_tac \\ gvs []
+    \\ reverse $ Cases_on ‘r’ \\ gvs []
+    >- (drule exp_ress_rel_rerr \\ rpt strip_tac \\ gvs [evaluate_def])
+    \\ drule exp_ress_rel_rval \\ rpt strip_tac \\ gvs [evaluate_def])
 QED
 
 val _ = export_theory ();
